removed config from keyschedule; we may need to add more specific parameters later

src/tls/HandshakeLog.fst
@@ -11,22 +11,43 @@ open TLSConstants
 open TLSInfo
 open HandshakeMessages
 
+val validLog: list hs_msg -> Tot bool
+let validLog hsl = 
+    match hsl with
+    | [] -> true
+    | [ClientHello ch] -> true
+    | (ClientHello ch) :: (ServerHello sh) :: rest -> true
+    | _ -> false
+
+val getLogVersion: hsl:list hs_msg{validLog hsl} -> Tot (option protocolVersion)
+let getLogVersion hsl =
+    match hsl with
+    | (ClientHello ch) :: (ServerHello sh) :: rest -> Some sh.sh_protocol_version
+    | _ -> None
+
 type log =
-     | LOG: pv: protocolVersion -> #region:rid -> rref region (hsl:list hs_msg & b:bytes{b = handshakeMessagesBytes pv hsl}) -> log 
+     | LOG: #region:rid -> logref:rref region (pv:option protocolVersion & hsl:list hs_msg & b:bytes{validLog hsl && getLogVersion hsl = pv && handshakeMessagesBytes pv hsl = b}) -> log 
 
-val init: pv:protocolVersion -> reg:rid -> log 
-let init pv reg = 
+val create: #reg:rid -> ST log
+  (requires (fun h -> True))
+  (ensures (fun h0 i h1 -> True))
+let create #reg = 
     let hsl: list hs_msg = [] in
-    let r = ralloc reg (|hsl,empty_bytes|) in
-    LOG pv #reg r 
+    let r = ralloc reg (|None,hsl,empty_bytes|) in
+    LOG #reg r 
 
-val append_log: log -> hs_msg -> bytes
-let append_log (LOG pv #reg lref) hm = 
-    let mb = handshakeMessageBytes pv hm in
-    let (|hsl,lb|) = !lref in 
+val append_log: l:log -> hm:hs_msg -> ST bytes
+    (requires (fun h ->
+	       let (|pv,hsl,lb|) = sel h l.logref in
+	       validLog (List.Tot.append hsl [hm])))
+    (ensures (fun h1 b h2 -> True))
+let append_log (LOG #reg lref) hm = 
+    let (|pv,hsl,lb|) = !lref in 
     let hsl' = FStar.List.Tot.append hsl [hm] in
+    let pv = getLogVersion hsl' in
+    let mb = handshakeMessageBytes pv hm in
     let lb' = lb @| mb in
-    lref := (|hsl',lb'|);
+    lref := (|pv,hsl',lb'|);
     mb
 
 let op_At_At l h = append_log l h
@@ -34,14 +55,14 @@ let op_At_At l h = append_log l h
 val getMessages: log -> ST (list hs_msg)
   (requires (fun h -> True))
   (ensures (fun h0 i h1 -> True))
-let getMessages (LOG pv #reg lref) = 
-    let (|hsl,lb|) = !lref in hsl
+let getMessages (LOG #reg lref) = 
+    let (|pv,hsl,lb|) = !lref in hsl
 
 val getBytes: log -> ST bytes 
   (requires (fun h -> True))
   (ensures (fun h0 i h1 -> True))
-let getBytes (LOG pv #reg lref) = 
-    let (|hsl,lb|) = !lref in lb
+let getBytes (LOG #reg lref) = 
+    let (|pv,hsl,lb|) = !lref in lb
 
 assume val checkLogSessionHash: list hs_msg -> csr:csRands -> pv:protocolVersion -> cs:cipherSuite -> negotiatedExtensions -> bool
 assume val checkLogClientFinished: list hs_msg -> csr:csRands -> pv:protocolVersion -> cs:cipherSuite -> negotiatedExtensions -> bool
